semantics/semanticPrimitivesScript.sml
@@ -93,6 +93,9 @@ val _ = Define `
 val _ = Define `
  (list_type_num : num= (( 1 : num)))`;
 
+val _ = Define `
+ (option_type_num : num= (( 2 : num)))`;
+
 
 (* The result of evaluation *)
 val _ = Hol_datatype `
